\documentclass[12pt]{article}
\input{common.tex}

\begin{document}
Let a linear map $\mathcal{T}$ map from $n$ dimensional vectors to $m$ dimensional vectors.
Let $\{\undertilde{e_i}\}$ be a basis of $n$ dimensional space and 
$\{\undertilde{f_i}\}$ be basis of $m$ dimensional space.
Thus, there exists $a_i,b_i$ such that

\[\undertilde{a} = a_{i} \undertilde{e_{i}}\]
\[\undertilde{b} = b_{i} \undertilde{f_{i}}\]

There must exist matrix $T$ corresponding to $\mathcal{T}$ such that $b_i = T_{ij}a_j$.
We claim that $T$ sends basis to basis.

\[ \begin{aligned}
        \mathcal{T}(\undertilde{a}) &= \undertilde{b} = b_j \undertilde{f_j}\\
        \mathcal{T}(a_j\undertilde{e_j}) &= T_{ji}a_i\undertilde{f_j}\\
        a_i\mathcal{T}(\undertilde{e_i}) &= T_{ji}a_i\undertilde{f_j}\\
\end{aligned} \]
From here, there are two ways to continue. 
Since $a_i$ are the components of arbitrary vector $\undertilde{a}$,
it is okay to divide by $a_i$ on both sides and yield
\[\mathcal{T}(\undertilde{e_i}) = T_{ji}\undertilde{f_j}\]
Thus proving the result. Alternatively, more directly,
let $a_i = \delta_{ik}$. Then,
\[\delta_{ik}\mathcal{T}(\undertilde{e_i}) = T_{ji}\delta_{ik}\undertilde{f_j}\]
\[\mathcal{T}(\undertilde{e_k}) = T_{jk}\undertilde{f_j}\]
which is the same conclusion.

Now consider new sets of basis $\{\undertilde{e'_{i}}\}$ and $\{\undertilde{f'_{j}}\}$, so that we have

\[\undertilde{a} = a'_{i}\undertilde{e'_{i}}\]
\[\undertilde{b} = b'_{i}\undertilde{e'_{i}}\]

Since $e_j$ and $f_j$ are bases, there exist matrices $P,Q$ such that
\[\undertilde{e'_{i}} = P_{ji}\undertilde{e_{j}}\]
\[\undertilde{f'_{j}} = Q_{kj}\undertilde{f_{k}}\]

Define matrix $T'$ corresponding to $\mathcal{T}$ under the new basis, i.e. such that
\[b'_{i} = T'_{ji}a'_{i}\]

We claim that it is possible to express $T'$ in terms of $T$, $P$, and $Q$.

By the previous part, we have

\[\mathcal{T}(\undertilde{e'_{i}}) = T'_{ji}\undertilde{f'_{j}}\]

substituting yields

\[\mathcal{T}(P_{ji}\undertilde{e_{j}}) = T'_{ji}Q_{kj}\undertilde{f_{k}}\]
\[P_{ji}\mathcal{T}(\undertilde{e_{j}}) = T'_{ji}Q_{kj}\undertilde{f_{k}}\]

and by the previous part again we have

\[P_{ji}T_{kj}\undertilde{f_k} = T'_{ji}Q_{kj}\undertilde{f_{k}}\]

Here we have that since $\undertilde{f_j}$ are a set of basis, they are linearly independent. Thus,

\[P_{ji}T_{kj} = T'_{ji}Q_{kj}\]
\[(TP)_{ik} = (QT')_{ik}\]
\[TP = QT'\]
\[T' = Q^{-1}TP\]

\end{document}
